spot/GC.SPOT.HeapExpansion.fst
@@ -1636,6 +1636,28 @@ let spot_chunked_cheney_promote_head_split_preserves_chunked_alloc_shape
   CheneyPreservation.chunked_cheney_promote_head_split_preserves_chunked_alloc_shape
     minor major fp roots alloc_fuel
 
+let spot_chunked_cheney_promote_head_split_preserves_old_major_objects
+  (minor: minor_state) (major: MH.major_heap) (fp: U64.t)
+  (roots: Seq.seq U64.t) (alloc_fuel: nat)
+  : Lemma
+      (requires
+        alloc_fuel > 1 /\
+        GenInv.chunked_major_alloc_shape major fp alloc_fuel /\
+        SpecMajorAlloc.major_fl_chain_terminates
+          major fp alloc_fuel = true /\
+        CheneyPreservation.chunked_cheney_promote_split_ready
+          minor major fp roots alloc_fuel)
+      (ensures
+        (let res =
+           ChunkedCheney.chunked_cheney_promote
+             minor major fp roots alloc_fuel in
+         forall (src: obj_addr).
+          Seq.mem src (MH.major_objects major) ==>
+          Seq.mem src (MH.major_objects res.major_final)))
+  =
+  CheneyPreservation.chunked_cheney_promote_head_split_preserves_old_major_objects
+    minor major fp roots alloc_fuel
+
 let spot_chunked_cheney_promote_head_split_preserves_chain_objects_blue
   (minor: minor_state) (major: MH.major_heap) (fp: U64.t)
   (roots: Seq.seq U64.t) (alloc_fuel: nat)
@@ -1749,6 +1771,9 @@ let spot_chunked_cheney_promote_after_minor_promotion_head_preflight
            Seq.mem x (minor_reachable minor roots) /\
            minor_wosize minor x > 0 ==>
            res.fwd_map x <> 0UL) /\
+         (forall (src: obj_addr).
+           Seq.mem src (MH.major_objects major) ==>
+           Seq.mem src (MH.major_objects res.major_final)) /\
          GenInv.chunked_major_alloc_shape
            res.major_final res.fp_final r.capacity_fuel_out /\
          SpecMajorAlloc.major_fl_chain_terminates
@@ -1831,6 +1856,11 @@ let spot_chunked_promote_object_head_split_preserves_chunked_alloc_shape
            res.major_out res.fp_out fuel = true /\
          (let alloc_res =
             SpecMajorAlloc.major_alloc_spec_with_fuel mh fp wosize fuel in
+          MH.major_objects res.major_out ==
+            MH.major_objects alloc_res.major_alloc_out /\
+          (forall (src:obj_addr).
+            Seq.mem src (MH.major_objects mh) ==>
+            Seq.mem src (MH.major_objects res.major_out)) /\
           Seq.mem (fp <: obj_addr)
             (MH.major_objects alloc_res.major_alloc_out) /\
           Seq.mem (fp <: obj_addr) (MH.major_objects res.major_out))))
@@ -3294,6 +3324,9 @@ let spot_chunked_cheney_collect_after_minor_promotion_head_preflight
            collect.cmc_major collect.cmc_fp r.capacity_fuel_out = true /\
          GenInv.chunked_chain_objects_blue
            collect.cmc_major collect.cmc_fp r.capacity_fuel_out /\
+         (forall (src: obj_addr).
+          Seq.mem src (MH.major_objects major) ==>
+          Seq.mem src (MH.major_objects collect.cmc_major)) /\
          (forall (x:U64.t).
           Seq.mem x (minor_reachable minor roots) /\
           minor_wosize minor x > 0 ==>
